proof/capDL-api/Invocation_DP.thy
@@ -282,6 +282,10 @@ lemma decode_asid_pool_invocation_inv[wp]:
    apply (wpc|wp |simp add:throw_on_none_def)+
   done
 
+crunch decode_vcpu_invocation, gen_decode_page_invocation, gen_decode_page_table_invocation
+  for inv[wp]: P
+  (simp: throw_on_none_def crunch_simps)
+
 lemma decode_invocation_inv[wp]:
   "\<lbrace>P\<rbrace> decode_invocation a b c d\<lbrace>\<lambda>_. P\<rbrace>, -"
   apply (simp add:decode_invocation_def)
